first draft nd test annotator

nonDeterministicTestGenerator.py
@@ -1,0 +1,184 @@
+#!/usr/bin/python
+import sys, getopt
+
+#works with predicates right now
+def findFunctionInFile(in_filename,origFnName):
+    fo = open(in_filename,"r+")
+    dafnyCode = fo.readlines()
+    count = 0
+    listofLines = []
+    foundStart = False
+    fullFnName = "predicate "+ origFnName
+    for line in dafnyCode:
+        args = line.split()
+        if(foundStart and line.strip()):   
+            listofLines.append(line.strip())
+        else:
+            foundStart = False
+        if(fullFnName in line):
+            listofLines.append(line.strip())
+            foundStart = True
+        count = count + 1
+    # print(listofLines)
+    return listofLines
+
+# returns:
+# (fullparams) == String of new and old parameters
+# (generatedPreConds) == List of strings, that are the new necessary pre conditions
+def handleSMParamsAndPreCond(parameters,origFnName):
+    #(ASSUME) 'next' state var is marked with " ' " notation
+    # print(parameters)
+    newParameters = []
+    partialNewParams = []
+    originalNextVar = []
+    fullparams = ""
+
+    for p in parameters:
+        if ("'" in p):
+            individualP = p.split(":")
+            partialNewParams.append(individualP[0]+"':"+individualP[1])
+            newParameters.append(individualP[0]+"':"+individualP[1])
+            originalNextVar.append(p)
+        else:
+            partialNewParams.append(p)
+     # put all params together
+    for origP in parameters:
+        fullparams = fullparams + origP + ","
+    for newP in newParameters:
+        fullparams = fullparams + newP + ","
+    fullparams = fullparams[:-1]
+    # generate template pre-conditions
+    generatedPreConds = []
+    generatedPreConds.append("requires " + origFnName + "(" + stripParameterTypes(parameters) + ")")
+    generatedPreConds.append("requires " + origFnName + "(" + stripParameterTypes(partialNewParams) + ")")
+    return fullparams,generatedPreConds, originalNextVar, newParameters
+
+# returns:
+# (fullparams) == String of new and old parameters
+# (generatedPreConds) == List of strings, that are the new necessary pre conditions
+# (oldParams) == List of original parameters
+# (newParams) == List of new parameters
+def handleNonSMParamsAndPreCond(parameters):
+    newParameters = []
+    fullparams = ""
+    for p in parameters:
+        individualP = p.split(":")
+        newParameters.append(individualP[0]+"':"+individualP[1])            
+    # put all params together
+    for origP in parameters:
+        fullparams = fullparams + origP + ","
+    for newP in newParameters:
+        fullparams = fullparams + newP + ","
+    fullparams = fullparams[:-1]
+    # generate template pre-conditions
+    generatedPreConds = []
+    for i in range(len(parameters)):
+        gPreCond = "requires " + parameters[i].split(":")[0] + " == " + newParameters[i].split(":")[0]
+        generatedPreConds.append(gPreCond)
+    return fullparams, generatedPreConds ,parameters, newParameters
+
+# returns:
+# (existingPreCond) == List of exisiting Pre Conditions 
+def handleExistingPreConditions(originalFn):
+    #Assuming no 'ensures', existing Requires are between params and start of body
+    indexOfBodyStart = originalFn.index("{")
+    existingPreCond = originalFn[1:indexOfBodyStart]
+    return existingPreCond
+
+#returns
+# (stripedParameters) == list of parameters stripped of their 'types'
+def stripParameterTypes(parameterList):
+    stripedParameters = ""
+    for p in parameterList:
+        stripedParameters = stripedParameters + p.split(":")[0] + ","
+    return stripedParameters[:-1]
+
+# creates lemma as a String
+def makeLemma(lemmaName,parameterList,preConds,postConds,body):
+    lemma = "lemma " + lemmaName + "(" + parameterList + ")"
+    for preC in preConds:
+        lemma = lemma + "\n\t" + preC
+    for postC in postConds:
+        lemma = lemma + "\n\t" + postC
+    lemma = lemma + "\n{\n\t\t" + body + "\n}"
+    return lemma
+
+def generateNDLemma(originalFn,origFnName,isStateTransPredicate):
+    lemmaName = "is_"+origFnName+"_ND"
+    fullparams = ""
+    generatedPreConds = []
+    existingPreCond = []
+    newPostCond = []
+    #handle parameters
+    parameters = originalFn[0].split("(")[1][:-1].split(",")
+    # CASE: Normal Predicate
+    if(not isStateTransPredicate):
+        fullparams,generatedPreConds,origParams,newParams = handleNonSMParamsAndPreCond(parameters)
+        # print("FULL PARAMS == ",fullparams)
+        # print("generatedPreConds == ",generatedPreConds)
+        #--handle existing pre-conditions--
+        existingPreCond = handleExistingPreConditions(originalFn)
+        # generate new post-condition
+        newPostCond.append("ensures " + origFnName + "(" + stripParameterTypes(origParams) + ") == " + origFnName + "(" + stripParameterTypes(newParams) + ")")
+        # put it all together
+    else:
+        fullparams,generatedPreConds,originalNextVar, newParameters = handleSMParamsAndPreCond(parameters,origFnName)
+         # generate new post-condition
+        newPostCond.append("ensures " + originalNextVar[0].split(":")[0] + " == " + newParameters[0].split(":")[0])
+    return makeLemma(lemmaName,fullparams,existingPreCond+generatedPreConds,newPostCond,"")
+
+def usage():
+    return ("nonDeterministicTestGenerator.py" + 
+                    "\n\t -i <inputfile> " +
+                    "\n\t -n <nameOfFunction> "+ 
+                    "\n\t -s StateMachineFlag(default=False): " + 
+                    "\n\t\t True: designated predicate is a state machine transition" + 
+                    "\n\t\t False: designated predicate is a standard predicate"+
+                    "\n\t -a AppendFlag(default=False): " + 
+                    "\n\t\t True: generated lemma is appended to bottom of input file" + 
+                    "\n\t\t False: generated lemma is only printed to console" )
+def main(argv):
+    inputfile = ''
+    outputfile = ''
+    nameOfFunction = ''
+    smFlag = False
+    appendFlag = False
+    try:
+        opts, args = getopt.getopt(argv,"hi:n:s:a:",["ifile=","noffun=","smFlag=","appendFlag="])
+    except getopt.GetoptError:
+        print(usage())
+        sys.exit(2)
+    for opt, arg in opts:
+        if opt == '-h':
+            print(usage())
+            sys.exit()
+        elif opt in ("-i", "--ifile"):
+            inputfile = arg
+        elif opt in ("-n", "--noffun"):
+            nameOfFunction = arg
+        elif opt in ("-s", "--smFlag"):
+            smFlag = arg
+        elif opt in ("-a", "--appendFlag"):
+            appendFlag = arg
+    print("======================================")
+    print('Input file is: ', inputfile)
+    print('Name of Function to test is: ', nameOfFunction)
+    print('StateMachineFlag: ', smFlag)
+    print('AppendFlag: ', appendFlag)
+    print("======================================\n")
+    
+
+    functionTxt = findFunctionInFile(inputfile,nameOfFunction)
+    lemma = generateNDLemma(functionTxt,nameOfFunction,smFlag)
+    print(lemma)
+
+    print("\n======================================\n")
+    if(appendFlag):
+        with open(inputfile, "a") as f:
+            f.write("\n"+lemma)
+        print("DONE: Appended to input file")
+    else:
+        print("DONE")
+
+if __name__ == "__main__":
+   main(sys.argv[1:])
