template.s.dfy
@@ -1,0 +1,67 @@
+datatype Constants = Constants(capacity:int)
+datatype CokeMachine = CokeMachine(numCokes:int)
+
+
+predicate pred<T(==)>(a:T,b:T)
+{
+    a == b
+}
+
+predicate divides(factor:nat, candidate:nat)
+  requires 1<=factor
+{
+  candidate % factor == 0
+}
+
+predicate StateTrans<C,V>(c:C,v:V,v':V)
+{
+  true
+}
+
+lemma isPredSM_ND<C,V>(c:C,v:V,v':V,v'':V)
+  requires StateTrans(c,v,v')
+  requires StateTrans(c,v,v'')
+//   ensures v' == v''
+//   {}
+
+predicate Purchase(c:Constants, v:CokeMachine, v':CokeMachine) {
+    && v.numCokes > 0
+    && v'.numCokes == v.numCokes - 1
+}
+
+predicate pre<T>(a:T){
+	true
+}
+
+predicate post<T>(a:T){
+	true
+}
+
+  lemma lemmaOrMethodThatReturnsAValue<T>(a:T) returns (b:T)
+    requires pre(a)
+    ensures post(b)
+
+  lemma isLemmaND<T>(a:T,a':T) returns (result:bool)
+    requires pre(a) && pre(a')
+    requires a == a'
+    // ensures result
+  {
+    var b := lemmaOrMethodThatReturnsAValue(a);
+    var b' := lemmaOrMethodThatReturnsAValue(a');
+    // return b == b';
+  }
+
+    predicate convertedPredicate<T>(a:T,b:T)
+    requires pre(a)
+  {
+    post(b)
+
+  }
+
+    lemma isConvertedLemmaorMethodND<T>(a:T,b:T,b':T)
+    requires pre(a)
+    requires convertedPredicate(a,b)
+    requires convertedPredicate(a,b')
+    // ensures b == b'
+    // {}
+  
